new/golang/defn/ffi.v
@@ -1,0 +1,74 @@
+From New Require Export notation.
+From New.golang.theory Require Import typing.
+From Perennial Require Import base.
+From Perennial.Helpers Require Import Transitions.
+
+Local Instance models_syntax : ffi_syntax :=
+  {|
+    ffi_opcode := (go_string * go_string);
+    ffi_val := Empty_set;
+  |}.
+
+Module model.
+  Record t :=
+    mk {
+        global_state : Type;
+        state : Type;
+        step : go_string -> val -> transition (state*global_state) expr;
+        crash_step : state -> state -> Prop;
+        #[global] state_inhabited :: Inhabited state;
+        #[global] global_state_inhabited :: Inhabited global_state;
+      }.
+End model.
+
+Class models : Type :=
+  {
+    model_names : gset go_string;
+    models_lookup : { model_name : go_string & (model_name ∈ model_names) } → model.t;
+  }.
+
+Section to_ffi.
+Context {M : models}.
+
+Local Notation model_names_type := { model_name : go_string & (model_name ∈ model_names) }.
+
+Definition models_state : Type :=
+  ∀ (name : model_names_type), (models_lookup name).(model.state).
+
+Definition models_global_state : Type :=
+  ∀ (name : model_names_type), (models_lookup name).(model.global_state).
+
+Program Instance models_ffi_model : ffi_model :=
+  {|
+    ffi_state := models_state;
+    ffi_global_state := models_global_state;
+  |}.
+Next Obligation.
+  refine (populate (fun _ => inhabitant)).
+Qed.
+Final Obligation.
+  refine (populate (fun _ => inhabitant)).
+Qed.
+
+Definition models_ffi_step :=
+  λ (op : ffi_opcode) (v : val),
+    let '(model_name, op_name) := op in
+    match decide (model_name ∈ model_names) with
+    | right _ =>  undefined
+    | left in_pf =>
+        let m := models_lookup (existT model_name in_pf) in
+        undefined
+        (* TODO: lift to [models] *)
+        (* m.(model.step) op_name v *)
+    end : transition (state * global_state) expr.
+
+Definition models_ffi_crash_step (s s' : models_state) :=
+  ∀ (m : model_names_type), (models_lookup m).(model.crash_step) (s m) (s' m).
+
+Instance models_ffi_semantics : ffi_semantics models_syntax _ :=
+  {|
+    ffi_step := models_ffi_step;
+    ffi_crash_step := models_ffi_crash_step;
+  |}.
+
+End to_ffi.
